move core_inv into handle_pts_to, strengthen init post

steel/Zeta.Steel.SafeMain.fst
@@ -5,11 +5,25 @@ module R = Steel.ST.Reference
 
 open Steel.ST.GenElim
 
-let state_ptr_inv_prop
+[@@__reduce__]
+let state_ptr_has_core_inv_false
+  (p: perm)
+: Tot vprop
+= pure (p == full_perm)
+
+[@@__reduce__]
+let state_ptr_has_core_inv_true
+  (state: R.ref M.top_level_state)
+: Tot vprop
+= exists_ (fun ps -> exists_ (fun ts -> R.pts_to state ps ts `star` M.core_inv ts))
+
+let state_ptr_has_core_inv
   (p: perm)
   (state: R.ref M.top_level_state)
-: Tot prop
-= R.is_null state ==> p == full_perm
+: Tot vprop
+= if R.is_null state
+  then state_ptr_has_core_inv_false p
+  else state_ptr_has_core_inv_true state
 
 [@@__reduce__]
 let state_ptr_inv0
@@ -17,7 +31,7 @@ let state_ptr_inv0
 : Tot vprop
 = exists_ (fun (p: perm) -> exists_ (fun (state: R.ref M.top_level_state) ->
     R.pts_to state_ptr p state `star`
-    pure (state_ptr_inv_prop p state)
+    state_ptr_has_core_inv p state
   ))
 
 let state_ptr_inv
@@ -34,6 +48,9 @@ type handle_t = {
 let create_handle () : STT handle_t emp (fun _ -> emp) =
   let state_ptr : R.ref (R.ref M.top_level_state) = R.alloc R.null in
   noop ();
+  rewrite
+    (state_ptr_has_core_inv_false full_perm)
+    (state_ptr_has_core_inv full_perm R.null);
   rewrite
     (state_ptr_inv0 state_ptr)
     (state_ptr_inv state_ptr);
@@ -57,7 +74,8 @@ assume val handle: handle_t
 let handle_pts_to0
   (ts: M.top_level_state)
 : Tot vprop
-= exists_ (fun p -> exists_ (fun r -> exists_ (fun p0 ->
+= M.core_inv ts `star`
+  exists_ (fun p -> exists_ (fun r -> exists_ (fun p0 ->
     R.pts_to handle.state_ptr p r `star`
     R.pts_to r p0 ts
   )))
@@ -66,6 +84,20 @@ let handle_pts_to
   (ts: M.top_level_state)
 : Tot vprop
 = handle_pts_to0 ts
+
+let handle_pts_to_core_inv_intro
+  ts
+= rewrite (handle_pts_to ts) (handle_pts_to0 ts);
+  let _ = gen_elim () in
+  M.core_inv_share ts;
+  rewrite (handle_pts_to0 ts) (handle_pts_to ts)
+
+let handle_pts_to_core_inv_elim
+  ts
+= rewrite (handle_pts_to ts) (handle_pts_to0 ts);
+  let _ = gen_elim () in
+  M.core_inv_gather ts;
+  rewrite (handle_pts_to0 ts) (handle_pts_to ts)
 
 let gather ts1 ts2 =
   rewrite (handle_pts_to ts1) (handle_pts_to0 ts1);
@@ -79,7 +111,9 @@ let gather ts1 ts2 =
   let r = vpattern_replace (R.pts_to handle.state_ptr _) in 
   vpattern_rewrite (fun (r: R.ref M.top_level_state) -> R.pts_to r p1 _) r;
   vpattern_rewrite (fun (r: R.ref M.top_level_state) -> R.pts_to r p2 _) r;
-  R.gather _ r;
+  R.gather p1 r;
+  rewrite (M.core_inv ts2) (M.core_inv ts1);
+  M.core_inv_gather ts1;
   rewrite (handle_pts_to0 ts1) (handle_pts_to ts1)
 
 let share
@@ -89,6 +123,7 @@ let share
   let r : R.ref M.top_level_state = vpattern_replace (fun r -> R.pts_to handle.state_ptr _ r `star` R.pts_to r _ ts) in
   R.share handle.state_ptr;
   R.share r;
+  M.core_inv_share ts;
   rewrite (handle_pts_to0 ts) (handle_pts_to ts);
   noop ();
   rewrite (handle_pts_to0 ts) (handle_pts_to ts)
@@ -96,32 +131,44 @@ let share
 #push-options "--z3rlimit 16"
 #restart-solver
 
-let init () : STT bool
-  emp
-  (fun b -> init_post b)
+let init ()
 = Lock.acquire handle.lock;
   rewrite (state_ptr_inv handle.state_ptr) (state_ptr_inv0 handle.state_ptr);
   let _ = gen_elim () in
   let state = R.read handle.state_ptr in
+  vpattern_rewrite (state_ptr_has_core_inv _) state;
+  let p = vpattern_replace (fun p -> state_ptr_has_core_inv p _) in
   if R.is_null state
   then begin
+    rewrite (state_ptr_has_core_inv _ _) (state_ptr_has_core_inv_false p);
+    let _ = gen_elim () in
     let state = M.init () in
     let ts = elim_exists () in
+    M.core_inv_share ts;
     R.pts_to_not_null state;
-    assert (state_ptr_inv_prop (half_perm full_perm) state);
     vpattern_rewrite (fun p -> R.pts_to handle.state_ptr p _) full_perm;
     R.write handle.state_ptr state;
     R.share handle.state_ptr;
+    R.share state;
+    rewrite (state_ptr_has_core_inv_true state) (state_ptr_has_core_inv (half_perm full_perm) state);
     rewrite (state_ptr_inv0 handle.state_ptr) (state_ptr_inv handle.state_ptr);
     Lock.release handle.lock;
     rewrite (handle_pts_to0 ts) (handle_pts_to ts);
-    rewrite init_post_true (init_post true);
+    rewrite (init_post_true ts) (init_post true ts);
     return true
   end else begin
-    noop ();
+    rewrite (state_ptr_has_core_inv _ _) (state_ptr_has_core_inv_true state);
+    let _ = gen_elim () in
+    let ts = vpattern_replace_erased (fun ts -> R.pts_to state _ ts `star` M.core_inv ts) in
+    R.share state;
+    M.core_inv_share ts;
+    rewrite (R.pts_to handle.state_ptr _ _) (R.pts_to handle.state_ptr p state);
+    R.share handle.state_ptr;
+    rewrite (state_ptr_has_core_inv_true state) (state_ptr_has_core_inv (half_perm p) state);
     rewrite (state_ptr_inv0 handle.state_ptr) (state_ptr_inv handle.state_ptr);
     Lock.release handle.lock;
-    rewrite emp (init_post false);
+    rewrite (handle_pts_to0 ts) (handle_pts_to ts);
+    rewrite emp (init_post false ts);
     return false
   end
 
@@ -140,7 +187,6 @@ let verify_log
                (output:U.larray U8.t out_len)
   : STT (option (v:V.verify_result { V.verify_result_complete len v }))
     (handle_pts_to t `star`
-     M.core_inv t `star`
      A.pts_to input log_perm log_bytes `star`
      A.pts_to output full_perm out_bytes `star`
      M.log_of_tid t tid entries)
@@ -152,6 +198,7 @@ let verify_log
   let state = R.read handle.state_ptr in
   vpattern_rewrite (R.pts_to handle.state_ptr _) state;
   vpattern_rewrite (fun (state: R.ref M.top_level_state) -> R.pts_to state _ t) state;
+  M.core_inv_share t;
   let res = M.verify_log state tid len input out_len output in
   rewrite (handle_pts_to0 t) (handle_pts_to t);
   return res
